A12Kernel.lean
@@ -72,6 +72,7 @@ import A12Kernel.Elaboration.Flat
 import A12Kernel.Elaboration.TemporalTargetPolicy
 import A12Kernel.Elaboration.TemporalComputationResult
 import A12Kernel.Elaboration.FullDateComputationApplication
+import A12Kernel.Elaboration.DateTimeComputationApplication
 import A12Kernel.Elaboration.FullDateComputation
 import A12Kernel.Elaboration.DateTimeComputation
 import A12Kernel.Elaboration.RawString
