A12Kernel/Proofs.lean
@@ -28,6 +28,7 @@ import A12Kernel.Proofs.DateTimeApplication
 import A12Kernel.Proofs.FullDateComputationResult
 import A12Kernel.Proofs.DateTimeComputationResult
 import A12Kernel.Proofs.FullDateComputationApplication
+import A12Kernel.Proofs.DateTimeComputationApplication
 import A12Kernel.Proofs.FullDateComputation
 import A12Kernel.Proofs.DateTimeComputation
 import A12Kernel.Proofs.Correlation
